Beth.sml
@@ -1,9 +1,482 @@
 
-val AX5 = store_ax("AX5",
-“!A.?B p:B->A Y M:B~>Y.  
- (!b Mb.
-     (?i:Mb->Y. Inj(i) & 
-                !y. (?y0. App(i,y0) = y) <=> Holds(M,b,y))
-     ==> P(App(p,b),Mb)) & 
- !a:mem(A) X. P(a,X) ==> ?b. App(p,b) = a”)
+(*member to relation*)
+val m2r_def = AX1 |> qspecl [‘A’,‘A’]
+                  |> fVar_sInst_th “P(x:mem(A),y:mem(A))”
+                  “IN(Pair(x,y),od:mem(Pow(A * A)))”
+                  |> uex2ex_rule 
+                  |> qSKOLEM "m2r" [‘od’] 
+                  |> qspecl [‘a1:mem(A)’,‘a2:mem(A)’]
+                  |> gen_all
 
+val r2m_def = 
+    IN_def_P |> qspecl [‘A * A’]
+             |> fVar_sInst_th “P(a12:mem(A * A))”
+             “Holds(R:A~>A,Fst(a12),Snd(a12))” 
+             |> uex2ex_rule 
+             |> qSKOLEM "r2m" [‘R’] 
+             |> qspecl [‘Pair(a1:mem(A),a2:mem(A))’]
+             |> rewr_rule [Pair_def']
+             |> gen_all
+
+
+val isleast_def = qdefine_psym("isleast",[‘R:A~>A’,‘s:mem(Pow(A))’,‘l:mem(A)’])
+‘IN(l,s) & !a. IN(a,s) ==> Holds(R,l,a)’
+
+val Well_def = qdefine_psym("Well",[‘R:A~>A’])
+‘Total(R) & 
+ !s. ~(s = Empty(A)) ==> ?l. isleast(R,s,l)’ 
+|> gen_all
+
+val INr_def = qdefine_psym("INr",[‘a:mem(A)’,‘R:A~>A’])
+‘?a1. Holds(R,a,a1) | Holds(R,a1,a)’
+
+(*why choose to define snocrel like this instead of using 
+A + 1, A + 1 + 1,... etc, 
+then do not need to inject into A, easier to take bigunion,
+
+and easier to say for every well order, for every base, instead of of certain form.
+
+
+Initially it was:
+“!A R:A~>A a.~INr(a,R) ==>
+ ?!Ra. !a1 a2. Holds(Ra,a1,a2) <=> 
+ Holds(R,a1,a2) | (INr(a1,R) & a2 = a)”
+
+but thhen realise do not need the precond to define the rel
+*)
+val snocrel_def = 
+AX1 |> qspecl [‘A’,‘A’] 
+    |> fVar_sInst_th “P(a1:mem(A),a2:mem(A))”
+    “ Holds(R:A~>A,a1,a2) | (INr(a1,R) & a2 = a)”
+    |> uex2ex_rule |> qSKOLEM "snocrel" [‘R’,‘a’]
+    |> qspecl [‘a1:mem(A)’,‘a2:mem(A)’]
+    |> gen_all
+
+(*member of power set to set,
+to prove uniqueness !!!!!*)
+val m2s_def = proved_th $
+e0
+(cheat)
+(form_goal “!X xs:mem(Pow(X)). ?X0 i:X0->X. 
+ Inj(i) & 
+ !x. IN(x,xs) <=> ?x0:mem(X0). x = App(i,x0)”)
+|> spec_all |> qSKOLEM "m2s" [‘xs’] 
+|> qSKOLEM "m2i" [‘xs’] |> gen_all
+
+(*inductive relaion need b is a member of some set B.
+  can prove each finite beth exist,
+ then the 
+*)
+
+val snocm_def = qdefine_fsym("snocm",[‘r:mem(Pow(A * A))’,‘a:mem(A)’]) ‘r2m(snocrel(m2r(r),a))’ 
+
+
+
+ 
+val ischain_def = 
+    qdefine_psym("ischain",
+                 [‘r:A~>A’,‘s:mem(Pow(A))’])
+    ‘!a1 a2. IN(a1,s) & IN(a2,s) ==> 
+     Holds(r,a1,a2) | Holds(r,a2,a1)’
+                           |> gen_all
+ 
+val SSr_def =  
+    AX1 |> qspecl [‘Pow(A)’,‘Pow(A)’]
+        |> fVar_sInst_th “P(s1:mem(Pow(A)),s2:mem(Pow(A)))”
+           “SS(s1:mem(Pow(A)),s2)”
+        |> uex2ex_rule |> qSKOLEM "SSr" [‘A’] 
+
+val SSchain_def = qdefine_psym("SSchain",
+[‘s:mem(Pow(Pow(A)))’]) ‘ischain(SSr(A),s)’
+|> gen_all
+
+local
+val iswo_cl = 
+ “(od = Empty(A * A) ==> IN(od,wo)) &
+  (!od0 a.
+      IN(od0,wo) & ~INr(a,m2r(od0)) & od = snocm(od0,a) 
+      ==> IN(od,wo)) &
+  (!s. (!od0. IN(od0,s) ==> IN(od0,wo)) & 
+       SSchain(s) &
+       od = BIGUNION(s) ==>
+   IN(od,wo)) ”
+in
+val (iswo_incond,x1) = mk_incond iswo_cl;
+val iswof_ex = mk_fex iswo_incond x1;
+val iswof_def = mk_fdef "iswof" iswof_ex;
+val iswof_monotone = proved_th $
+e0
+(cheat)
+(form_goal 
+“!s1 s2.SS(s1,s2) ==> 
+  SS(App(iswof(A), s1), App(iswof(A), s2))”)
+val iswo's_def = mk_prim iswof_def;
+val iswos_def = mk_LFP (rastt "iswo's(A)");
+val iswos_cond = mk_cond iswos_def iswo's_def;
+val iswos_SS = mk_SS iswos_def iswo's_def;
+val iswo_rules0 = mk_rules iswof_monotone iswos_SS iswos_cond;
+val iswo_cases0 = mk_cases iswof_monotone iswo_rules0 iswos_cond;
+val iswo_ind0 = mk_ind iswos_cond;
+val iswo_ind1 = mk_ind1 iswof_def iswo_ind0;
+val iswo_ind2 = mk_ind2 iswo_ind1;
+val iswo_cases1 = mk_case1 iswof_def iswo_cases0;
+val iswo_rules1 = mk_rules1 iswof_def iswo_rules0;
+val iswo_rules2 = mk_rules2 iswo_rules1;
+val iswo_rules3 = mk_rules3 iswo_rules2;
+end
+ 
+val iswo_ind = iswo_ind2 |> store_as "iswo_ind";
+val iswo_cases = iswo_cases1 |> store_as "iswo_cases";
+val iswo_rules = iswo_rules3 |> store_as "iswo_rules";
+
+val WO_def = Thm_2_4 |> qspecl [‘Pow(A * A)’] 
+                    |> fVar_sInst_th 
+                       “P(od:mem(Pow(A * A)))” 
+                       “IN(od:mem(Pow(A * A)),iswos(A))”
+                    |> qSKOLEM "WO" [‘A’] 
+                    |> qSKOLEM "iWO" [‘A’]
+                    |> gen_all
+
+val Rwo_iswos = prove_store("Rwo_iswos",
+e0
+(rpt strip_tac >> 
+ assume_tac
+ (WO_def|> spec_all 
+                      |> conjE2 
+                      |> qspecl [‘Rwo(wo:mem(WO(A)))’]
+                      |> rewr_rule[GSYM Rwo_def]) >>
+ arw[] >> qexists_tac ‘wo’ >> rw[])
+(form_goal “!A wo. IN(Rwo(wo), iswos(A))”));
+
+
+
+(*if as constructors, will have 
+O | Suc ord | U (ord set)
+!!!!!!!!! *)
+val Rwo_def = qdefine_fsym("Rwo",[‘wo:mem(WO(A))’])
+‘App(iWO(A),wo)’ |> gen_all
+
+val zord_def = proved_th $
+e0
+(rpt strip_tac >> rw[Rwo_def] >>
+ irule $ iffRL Inj_ex_uex >>
+ rw[WO_def] >> flip_tac >> rw[GSYM WO_def] >>
+ rw[iswo_rules])
+(form_goal “!A. ?!zo. Rwo(zo) = Empty(A * A)”)
+|> spec_all |> uex2ex_rule |> qSKOLEM "zord" [‘A’]
+|> gen_all
+
+val wo_ex = proved_th $
+e0
+(strip_tac >> qexists_tac ‘zord(A)’ >> rw[])
+(form_goal “!A. ?wo:mem(WO(A)).T”)
+
+val sord_def = proved_th $
+e0
+(cheat)
+(form_goal 
+ “!A wo a:mem(A). ~INr(a,m2r(Rwo(wo))) ==>
+  ?!wo1.Rwo(wo1) = snocm(Rwo(wo),a)”)
+|> spec_all |> undisch |> uex2ex_rule 
+|> SKOLEM (spec_all wo_ex) "sord" 
+[("wo",mem_sort (rastt "WO(A)")),
+ ("a",mem_sort (rastt "A"))]
+|> disch_all |> gen_all
+
+
+(*add the condition of being an infinite chain?*)
+val lord_def = proved_th $
+e0
+(cheat)
+(form_goal 
+ “!A s. SSchain(IMAGE(iWO(A),s)) ==>
+  ?!lo.Rwo(lo) = BIGUNION(IMAGE(iWO(A),s))”)
+|> spec_all |> undisch |> uex2ex_rule 
+|> SKOLEM (spec_all wo_ex) "lord" 
+[("s",mem_sort (rastt "Pow(WO(A))"))]
+|> disch_all |> gen_all
+
+val Leo_def = qdefine_psym("Leo",[‘wo1:mem(WO(A))’,‘wo2:mem(WO(A))’]) ‘SS(Rwo(wo1),Rwo(wo2))’ |> gen_all
+
+val LEo_def = 
+    AX1 |> qspecl [‘WO(A)’,‘WO(A)’] 
+        |> fVar_sInst_th “P(a:mem(WO(A)),b:mem(WO(A)))”
+           “Leo(a:mem(WO(A)),b)”
+        |> uex2ex_rule |> qSKOLEM "LEo" [‘A’]
+        |> store_as "LEo_def";
+
+val all_P_WO = prove_store("all_P_WO",
+e0
+(dimp_tac >> rpt strip_tac >> arw[] >>
+ first_x_assum (qspecl_then [‘Rwo(wo)’] assume_tac) >>
+ fs[Rwo_iswos] >>
+ first_x_assum irule >> rw[])
+(form_goal
+ “(!wo:mem(WO(A)).P(wo)) <=> 
+  (!od:mem(Pow(A * A)). IN(od,iswos(A)) ==>
+    IN(od,iswos(A)) & 
+    (!wo.Rwo(wo) = od ==> P(wo)))
+  ”));
+
+(*
+val ind = iswo_ind
+*)
+
+fun mk_induct ind = 
+    let val (svar as (n,s),b) = dest_forall (concl ind) 
+        val st = mk_var svar
+        val pset = s |> dest_sort |> #2 |> hd
+                     |> dest_fun |> #3 |> hd
+        val specindefp = IN_def_P_ex |> allE pset
+        val (exv,exb) = dest_exists (concl specindefp)
+        val specind = ind |> allE (mk_var exv)
+        val ind' = rewr_rule[GSYM(assume exb)] 
+                            (add_assum exb specind) 
+    in existsE exv specindefp ind'
+    end
+
+val iswo_induct = mk_induct iswo_ind
+
+val Rwo_Empty_iff_zord = prove_store("Rwo_Empty_iff_zord",
+e0
+(rw[GSYM zord_def,Rwo_def] >>
+ rpt strip_tac >> irule Inj_eq_eq >>
+ rw[WO_def])
+(form_goal “!A wo.Rwo(wo) = Empty(A * A) <=> 
+ wo = zord(A)”));
+
+val iswo_snocm = iswo_rules |> conjE2 
+                            |> conjE1 
+
+
+val iswo_BIGUNION = iswo_rules |> conjE2 
+                               |> conjE2
+
+val iswo_Rwo = WO_def |> spec_all |> conjE2
+                      |> rewr_rule[GSYM Rwo_def]
+                      |> store_as "iswo_Rwo";
+
+val Rwo_snocm_iff_sord = prove_store("Rwo_snocm_iff_sord",
+e0
+(cheat)
+(form_goal “!A wo0 wo a:mem(A).Rwo(wo) = snocm(Rwo(wo0),a) <=> 
+ wo = sord(wo0,a)”));
+
+val all_wo_IMAGE = prove_store("all_wo_IMAGE",
+e0
+()
+(form_goal “SSchain(s) & Rwo(wo) = BIGUNION(s) <=> 
+ wo = lord(PREIM())”));
+
+
+val wo_induct = prove_store("wo_induct",
+e0
+(strip_tac >> disch_tac >>
+ match_mp_tac $ iffRL all_P_WO >>
+ ind_with iswo_induct >>
+ rw[iswo_rules,Rwo_Empty_iff_zord] >> 
+ strip_tac (* 2 *)
+ >-- (strip_tac (* 2 *)
+     >-- (rpt strip_tac >> arw[]) >>
+     rpt gen_tac >> strip_tac >>
+     qby_tac ‘IN(snocm(od0, a'), iswos(A))’ 
+     >-- (irule iswo_snocm >> arw[]) >> arw[] >>
+     rpt strip_tac >> fs[iswo_Rwo] >> 
+     qby_tac ‘P(b)’ 
+     >-- (first_x_assum irule >> arw[]) >>
+     qsuff_tac ‘wo = sord(b,a')’
+     >-- (strip_tac >> arw[] >>
+         last_x_assum irule >> arw[]) >>
+     rw[GSYM Rwo_snocm_iff_sord] >> rfs[]) >>
+ strip_tac >> strip_tac >> 
+ qby_tac
+ ‘IN(BIGUNION(s'), iswos(A))’
+ >-- (irule iswo_BIGUNION >> arw[] >>
+     rpt strip_tac >> 
+     first_x_assum drule >> arw[]) >> arw[] >>
+ rpt strip_tac >>
+ qsuff_tac 
+ ‘?ods. wo = lord(ods) &
+        ischain(LEo(A),ods) &
+        IMAGE(iWO(A),ods) = s'’
+ >-- (rpt strip_tac >> arw[] >>
+     last_x_assum strip_assume_tac >>
+     first_x_assum irule >> arw[] >>
+     rpt strip_tac >>
+     qsuff_tac ‘?od0. IN(od0,s') & Rwo(od) = od0’ 
+     >-- (strip_tac >> 
+          last_x_assum drule >> 
+          pop_assum strip_assume_tac >>
+          first_x_assum irule >>
+          arw[]) >>
+     qpick_x_assum ‘IMAGE(iWO(A), ods) = s'’ 
+     mp_tac >> rw[GSYM IN_EXT_iff,IMAGE_def] >>
+     strip_tac >> rw[IN_EXT_iff] >>
+     fs[GSYM Rwo_def,IN_EXT_iff] >>
+     qby_tac ‘?a. IN(a,ods) & Rwo(od) = Rwo(a)’ 
+     >-- (qexists_tac ‘od’ >> arw[]) >>
+     first_x_assum (drule o iffLR) >>
+     qexists_tac ‘Rwo(od)’ >> arw[]) >>
+cheat)
+(form_goal 
+ “!A. P(zord(A)) &
+      (!od a:mem(A). P(od) ==> P(sord(od,a))) &
+      (!ods. ischain(LEo(A),ods) &
+             (!od.IN(od,ods) ==> P(od))
+             ==> P(lord(ods))) ==>
+      !wo:mem(WO(A)).P(wo)”));
+
+val msEqv_def = qdefine_psym("msEqv",[‘s:mem(Pow(A))’,‘S’])
+‘Eqv(m2s(s),S)’ |> gen_all
+
+
+
+local
+val isbeth_cl = 
+ “(!s. Eqv(m2s(s),N) & p = Pair(zord(A),s) ==>
+      IN(p,beths)) & 
+  (!p0 s a. IN(p0,beths) & 
+            Eqv(m2s(s),Pow(m2s(Snd(p0)))) &
+          p = Pair(sord(Fst(p0),a),s) ==>
+          IN(p,beths)) &
+  (!ps. (!p.IN(p,ps) ==> IN(p,beths)) &
+        SSchain(IMAGE(iWO(A) o p1(WO(A),Pow(B)),ps)) &
+        p = Pair(lord(IMAGE(p1(WO(A),Pow(B)),ps)),
+                 BIGUNION(IMAGE(p2(WO(A),Pow(B)),ps))) ==>
+   IN(p,beths))”
+in
+val (isbeth_incond,x1) = mk_incond isbeth_cl;
+val isbethf_ex = mk_fex isbeth_incond x1;
+val isbethf_def = mk_fdef "isbethf" isbethf_ex;
+val isbethf_monotone = proved_th $
+e0
+(cheat)
+(form_goal 
+“!s1 s2.SS(s1,s2) ==> 
+  SS(App(isbethf(A,B), s1), App(isbethf(A,B), s2))”)
+val isbeth's_def = mk_prim isbethf_def;
+val isbeths_def = mk_LFP (rastt "isbeth's(A,B)");
+val isbeths_cond = mk_cond isbeths_def isbeth's_def;
+val isbeths_SS = mk_SS isbeths_def isbeth's_def;
+val isbeth_rules0 = mk_rules isbethf_monotone isbeths_SS isbeths_cond;
+val isbeth_cases0 = mk_cases isbethf_monotone isbeth_rules0 isbeths_cond;
+val isbeth_ind0 = mk_ind isbeths_cond;
+val isbeth_ind1 = mk_ind1 isbethf_def isbeth_ind0;
+val isbeth_ind2 = mk_ind2 isbeth_ind1;
+val isbeth_cases1 = mk_case1 isbethf_def isbeth_cases0;
+val isbeth_rules1 = mk_rules1 isbethf_def isbeth_rules0;
+val isbeth_rules2 = mk_rules2 isbeth_rules1;
+val isbeth_rules3 = mk_rules3 isbeth_rules2;
+end
+ 
+val isbeth_ind = isbeth_ind2 |> store_as "isbeth_ind";
+val isbeth_cases = isbeth_cases1 |> store_as "isbeth_cases";
+val isbeth_rules = isbeth_rules3 |> store_as "isbeth_rules";
+
+val isBeth_def = qdefine_psym("isBeth",[‘wo:mem(WO(A))’,‘s’]) ‘?B beth:mem(Pow(B)). IN(Pair(wo,beth),isbeths(A,B)) & msEqv(beth,s)’
+|> gen_all
+
+val msEqv_Whole = prove_store("msEqv_Whole",
+e0
+(cheat)
+(form_goal “!A. msEqv(Whole(A), A) ”));
+
+ 
+val msEqv_m2s = prove_store("msEqv_m2s",
+e0
+(cheat)
+(form_goal “!A s. msEqv(s:mem(Pow(A)), m2s(s)) ”));
+
+
+val Eqv_m2s = prove_store("Eqv_m2s",
+e0
+cheat
+(form_goal “!A.Eqv(m2s(Whole(A)), A)”));
+
+val isbeth_zord = isbeth_rules |> conjE1 
+val isbeth_sord = 
+isbeth_rules |> conjE2 |> conjE1
+             |> strip_all_and_imp
+             |> gen_all 
+             |> disch “Eqv(m2s(s:mem(Pow(B))), Pow(m2s(Snd(p0: mem(WO(A) * Pow(B))))))”
+             |> gen_all
+             |> disch_all |> qgen ‘p0’
+             |> qspecl 
+             [‘Pair(wo:mem(WO(A)),b:mem(Pow(B)))’]
+             |> rewr_rule[Pair_def']
+             |> undisch |> spec_all |> rewr_rule[Pair_def'] 
+  
+(*
+
+!(s : mem(Pow(B))).
+               Eqv(m2s(s#), Pow(m2s(Snd(Pair(od, beth))))) ==>
+               !(a' : mem(A)). IN(Pair(sord(od, a'#), s#), isbeths(A, B))
+
+*)
+
+(*if A can be injected into B , then Pow(A) can be injected into Pow(B)?*)
+val Beth_ex = prove("Beth_ex",
+e0
+(strip_tac >> ind_with (wo_induct |> spec_all) >>
+ strip_tac (* 2 *)
+ >-- (qexists_tac ‘N’ >> rw[isBeth_def] >>
+     qexistsl_tac [‘N’,‘Whole(N)’] >> 
+     rw[msEqv_Whole] >> irule isbeth_zord >>
+     rw[Eqv_m2s]) >>
+ strip_tac (* 2 *)
+ >-- rpt strip_tac >> fs[isBeth_def] >>
+     qby_tac
+     ‘?beth'. IN(Pair(od, beth'), isbeths(A, Pow(B))) ’
+     (*image of injection of beth into Pow*)
+     >-- cheat >>
+     pop_assum strip_assume_tac >>
+     drule isbeth_sord >> 
+     qby_tac
+      ‘!s:mem(Pow(Pow(B))). Eqv(m2s(s), Pow(m2s(Snd(Pair(od, beth'))))) <=> 
+        Eqv(m2s(s), Pow(m2s(beth')))’ 
+     >-- cheat >>
+     fs[] >> pop_assum (K all_tac) >>
+     qsuff_tac
+     ‘?s:mem(Pow(Pow(B))). Eqv(m2s(s), Pow(m2s(beth')))’
+     >-- (strip_tac >>
+     qexistsl_tac [‘m2s(s')’,‘Pow(B)’,‘s'’] >>
+     rw[msEqv_m2s] >>
+     fs[Pair_def'] >>
+     first_x_assum irule >> arw[]) >>
+     
+
+      )
+(form_goal 
+“!A wo:mem(WO(A)). ?s. isBeth(wo,s)”));
+(*
+
+Beth(wo:mem(Pow(A * A)),s:set) <=>
+?B b:mem(Pow(B)). beth0(wo,b) & Eqv(s,Asset(b))
+
+Beth(wo:mem(Pow(A * A)),b:mem(Pow(B)))
+
+Eqv(Asset(s),N) ==> beth0({},s) &
+
+require a is not in wo0
+beth0(wo0,s0) & wo = snocrel(wo0,a) & 
+Eqv(Asset(s),Pow(Asset(s0))) ==>
+beth0(wo,s) &
+
+(*wo is not a successor ordinal, but still well order*)
+(!wo0 a. ~wo = snocrel(wo,a) & WO(wo)) &
+
+(* f indexes a family of wo-beth number relation*)
+!J f:J->Pow(A * A) * Pow(B). 
+ (!j:mem(J). beth0(f(j)) & 
+  (!wo0. wo0 ⊆ wo & wo0 <> wo <=> ?j. Fst(f(j)) = wo0)) &
+
+(* s is the sup of the set of beth numbers indexed by J*)
+
+(!s0 j.Snd(App(f,j)) = s0 ==> Card(s0) <= Card(s)) &
+(!s'. (!s0 j.Snd(App(f,j)) = s0 ==> Card(s0) <= Card(s')) ==>
+ Card(s) <= Card(s') ) ==>
+
+beth(wo,s)
+
+
+*)
