quo.sml
@@ -3,20 +3,77 @@ val resp1_def = qdefine_psym("resp1",[‘f:A->B’,‘R:A~>A’]) ‘resp(f,R,id
 
 val resp1_property = prove_store("resp1_property",
 e0
-cheat
-(form_goal “!A B f:A->B R. resp(f,R,id(B)) <=> 
+(rpt strip_tac >> rw[resp1_def,resp_def,id_def])
+(form_goal “!A B f:A->B R. resp1(f,R) <=> 
  (!a1 a2. Holds(R,a1,a2) ==> App(f,a1) = App(f,a2))”));
 
 val Inj_INV = prove_store("Inj_INV",
 e0
-cheat
+(rpt strip_tac >>
+ assume_tac
+ (P2fun_uex |> qspecl [‘B’,‘A’] 
+ |> fVar_sInst_th “P(x:mem(B),y:mem(A))”
+    “App(f:A->B,y) = x |
+     (!a. ~(App(f,a) = x)) & y = a0”) >>
+ qby_tac
+ ‘!x. ?!y. 
+  App(f:A->B,y) = x |
+     (!a. ~(App(f,a) = x)) & y = a0’
+ >-- (strip_tac >> uex_tac >>
+     qcases ‘?a. App(f,a) = x’ (* 2 *)
+     >-- (fs[] >> qexists_tac ‘a’ >> arw[] >>
+         rpt strip_tac >> fs[Inj_def]  >>
+         first_x_assum irule >> arw[]) >>
+     qby_tac ‘!a. ~(App(f,a) = x)’ 
+     >-- (strip_tac >> ccontra_tac >>
+          qby_tac ‘?a. App(f,a) = x’ 
+          >-- (qexists_tac ‘a’ >> arw[]) >>
+          rfs[]) >>
+     qexists_tac ‘a0’ >> arw[]) >>
+ first_x_assum drule >>
+ qsuff_tac
+ ‘?ivf:B->A. ivf o f = Id(A) & 
+ (!b.(!a. ~(App(f,a) = b)) ==> App(ivf,b) = a0)’
+ >-- (strip_tac >> uex_tac >>
+     qexists_tac ‘ivf’ >> arw[] >>
+     rpt strip_tac >> rw[GSYM FUN_EXT] >> strip_tac >>
+     qcases ‘?a1.App(f,a1) = a’ (*  2 *)
+     >-- (pop_assum (strip_assume_tac  o GSYM)>> 
+         arw[GSYM App_App_o]) >>
+     qby_tac ‘!a1. ~(App(f,a1) = a)’ 
+     >-- (strip_tac >> ccontra_tac >>
+          qby_tac ‘?a1. App(f,a1) = a’ 
+          >-- (qexists_tac ‘a1’ >> arw[]) >>
+          rfs[]) >>
+     first_x_assum drule >>
+     first_x_assum drule >> arw[]) >>
+ pop_assum (strip_assume_tac o uex2ex_rule) >>
+ qexists_tac ‘f'’ >> rpt strip_tac (* 2 *)
+ >-- (rw[GSYM FUN_EXT] >> strip_tac >>
+     first_x_assum (qspecl_then [‘App(f,a)’] assume_tac) >>
+     fs[] (* 2 *)
+     >-- (fs[Inj_def] >> first_x_assum drule >>
+         arw[App_App_o,Id_def]) >>
+     first_x_assum (qspecl_then [‘a’] assume_tac) >>
+     fs[]) >>
+ first_x_assum (qspecl_then [‘b’] strip_assume_tac) >>
+ rfs[])
 (form_goal “!A B f:A->B. Inj(f) ==>
- !a0:mem(A). ?!ivf:B->A.!b.(!a.App(f,a) = b ==> App(ivf,b) = a) &
- ((!a. ~(App(f,a) = b)) ==> App(ivf,b) = a0)”));
+ !a0:mem(A). ?!ivf:B->A. ivf o f = Id(A) & 
+ (!b.(!a. ~(App(f,a) = b)) ==> App(ivf,b) = a0)”));
 
 val fun_mem_ex = proved_th $
 e0
-cheat
+(rpt strip_tac >>
+ assume_tac
+ (P2fun |> qspecl [‘B’,‘A’]
+ |> fVar_sInst_th “P(b:mem(B),a:mem(A))” “a = a0:mem(A)”) >>
+ qby_tac ‘!x:mem(B). ?!y. y = a0’ 
+ >-- (strip_tac >> uex_tac >> qexists_tac ‘a0’ >> rw[]) >>
+ first_x_assum drule >>
+ pop_assum strip_assume_tac >>
+ qexists_tac ‘f’ >> arw[]
+ )
 (form_goal “!A a0:mem(A) B. ?f:B->A.T”)
 
 
@@ -38,10 +95,9 @@ val Inj_LINV = prove_store("Inj_LINV",
 e0
 (rpt strip_tac >>
  rw[GSYM FUN_EXT,Id_def,App_App_o] >> drule LINV_def >>
- strip_tac >>
- first_x_assum (qspecl_then [‘a’,‘App(f,a')’] 
- strip_assume_tac) >>
- first_x_assum irule >> rw[])
+ strip_tac >> 
+ first_x_assum (qspecl_then [‘a’] strip_assume_tac) >>
+ arw[GSYM App_App_o,Id_def])
 (form_goal “!A B f:A->B.Inj(f) ==> !a.LINV(f,a) o f = Id(A)”));
 
 val Abs_Surj = prove_store("Abs_Surj",
@@ -153,6 +209,17 @@ e0
   ?!fb: Q -> B. !a. 
   App(fb,abs(R,i,q0,a)) = App(f,a)”));
 
+
+
+
+(*
+val Qc_def = Thm_2_4 |> qspecl [‘Pow(G)’]
+                    |> fVar_sInst_th “P(s:mem(Pow(G)))”
+                    “?a. s = rsi(cstR(g,H:mem(Pow(G))),a)”
+                    |> qSKOLEM "Qc" [‘g’,‘H’]
+                    |> qSKOLEM "iQc" [‘g’,‘H’]
+                    |> store_as "Qc_def";
+
 val mem_Qc_e = prove_store("mem_Qc_e",
 e0
 (rpt strip_tac >> 
@@ -171,8 +238,82 @@ val ecst_def = mem_Qc_e |> spec_all |> uex2ex_rule
                         |> qSKOLEM "ecst" [‘g’,‘H’]
                         |> gen_all
 
+
+
+
 (*group quotient map *)
 val gqm_def = qdefine_fsym("gqm",[‘g:mem(Grp(G))’,‘H:mem(Pow(G))’]) ‘Abs(cstR(g,H),iQc(g,H),ecst(g,H))’
+
+(*As coset*)
+val Ascs_def = qdefine_fsym("Ascs",[‘g:mem(Grp(G))’,‘H:mem(Pow(G))’]) 
+‘LINV(iQc(g,H),ecst(g,H))’
+
+
+(*quotient group transpost *)
+val Qctp_def = qdefine_fsym("Qctp",[‘g:mem(Grp(G))’,‘H1:mem(Pow(G))’,‘H2:mem(Pow(G))’]) ‘LINV(iQc(g,H2),ecst(g,H2)) o iQc(g,H1)’
+
+val Rcs_Csof = prove_store("Rcs_Csof",
+e0
+cheat
+(form_goal 
+ “!G g H a:mem(G).Rcs(Csof(g, H, a)) = rsi(cstR(g, H), a)”));
+
+val Qctp_property = prove_store("Qctp_property",
+e0
+(rpt strip_tac >>
+ rw[Qctp_def,App_App_o,GSYM Rcs_def,Rcs_Csof] >>
+ arw[] >> 
+ rw[GSYM Rcs_Csof,Rcs_def,GSYM App_App_o] >>
+ qsspecl_then [‘H2’,‘g’] assume_tac iQc_Inj >>
+ drule Inj_LINV >> arw[Id_def])
+(form_goal
+ “!G g H1 H2:mem(Pow(G)).
+  H1 = H2 ==> 
+  !a.App(Qctp(g,H1,H2),Csof(g,H1,a)) = Csof(g,H2,a)”));
+
+val Qc_of_equal = prove_store("Qc_of_equal",
+e0
+(rpt strip_tac (* 2 *)
+ >-- (drule Qctp_property >>
+     rw[GSYM FUN_EXT,Id_def,App_App_o] >>
+     strip_tac >> 
+     qsspecl_then [‘g’,‘H2’] assume_tac gqm_Surj >>
+     fs[Surj_def] >>
+     first_assum 
+     (qspecl_then [‘a’]
+                  (x_choose_then "x" (assume_tac o GSYM))) >>
+     arw[gqm_Csof] >>
+     last_x_assum (assume_tac o GSYM) >>
+     drule Qctp_property >>
+     arw[]) >>
+ cheat )
+(form_goal “!G H1 H2:mem(Pow(G)).
+ H1 = H2 ==> 
+ !g.Qctp(g,H1,H2) o Qctp(g,H2,H1) = Id(Qc(g,H2)) &
+ Qctp(g,H2,H1) o Qctp(g,H1,H2) = Id(Qc(g,H1))”));
+
+val Qctp_ghom = prove_store("Qctp_ghom",
+e0
+(rpt strip_tac >> 
+ (*if arw[] here, then cannot make any change *)
+ rw[ghom_def] >> rpt strip_tac >>
+ qsspecl_then [‘g’,‘H1’] assume_tac gqm_Surj >>
+ fs[Surj_def] >>
+ first_assum 
+     (qspecl_then [‘a’]
+                  (x_choose_then "x" (assume_tac o GSYM))) >>
+     arw[gqm_Csof] >>
+ first_assum 
+     (qspecl_then [‘b’]
+                  (x_choose_then "y" (assume_tac o GSYM))) >>
+     arw[gqm_Csof] >>
+ drule Qctp_property >> arw[] >>
+ last_x_assum (assume_tac o GSYM) >>
+ drule Qctp_property >> arw[] >>
+ rw[gmul_Qg] >> arw[])
+(form_goal
+ “!G g H1 H2:mem(Pow(G)).
+ H1 = H2 ==> ghom(Qctp(g,H1,H2),Qg(g,H1),Qg(g,H2))”));
 
 val Quot_cstR_iQc = prove_store("Quot_cstR_iQc",
 e0
@@ -196,14 +337,6 @@ val gqm_Csof = prove_store("gqm_Csof",
 e0
 cheat
 (form_goal “!G g H a:mem(G). App(gqm(g,H),a) = Csof(g,H,a)”));
-
-val gmul_ginv = prove_store("gmul_ginv",
-e0
-cheat
-(form_goal 
-     “!G g:mem(Grp(G)) a.
-              gmul(g,ginv(g,a),a)= eof(g) &
-              gmul(g,a,ginv(g,a))= eof(g)”));
 
 val ghom_e = prove_store("ghom_e",
 e0
@@ -285,6 +418,207 @@ e0
  ghom(phi, Qg(g1,ker(f,g1,g2)), g2) &
  phi o gqm(g1,ker(f,g1,g2)) = f”));
 
+(*
+
+“H1 = H2 ==> LINV(iQc(g,H2)) o iQc(g,H1)
+ Abs Rep
+ Qc(g,H1) -> Qc(g,H2) ”
+
+*)
+
+val first_iso_thm = prove_store("first_iso_thm",
+e0
+(rpt strip_tac >>
+ qabbrev_tac ‘ker(f, g1, g2) = K’ >>
+ (* if arw[] then no change*)(*
+ qby_tac
+ ‘!phi:Qc(g1,ker(f, g1, g2)) -> G2.
+    (Inj(phi) &
+    ghom(phi, Qg(g1, ker(f, g1, g2)), g2) &
+    phi o gqm(g1, ker(f, g1, g2)) = f) <=> 
+   (Inj(phi o Qctp(g1,K,ker(f, g1, g2))) &
+     ghom(phi o Qctp(g1,K,ker(f, g1, g2)), Qg(g1, K), g2) &
+    phi o Qctp(g1,K,ker(f, g1, g2)) o gqm(g1, K) = f)’ 
+ >-- cheat >> 
+ qby_tac
+ ‘!phi:Qc(g1,ker(f, g1, g2)) -> G2.
+  ?psi:Qc(g1,K) -> G2. 
+   phi = psi o Qctp(g1,ker(f, g1, g2),K)’
+ >-- cheat >>
+ qby_tac
+ ‘!psi:Qc(g1,K) -> G2.
+  ?phi:Qc(g1,ker(f, g1, g2)) -> G2. 
+   psi = phi o Qctp(g1,K,ker(f, g1, g2))’
+ >-- cheat >>
+ qby_tac
+ ‘?!psi. Inj(psi) &
+  ghom(psi,Qg(g1,K),g2) &
+  psi o gqm(g1,K) = f’
+ >-- cheat >> *)
+ qsuff_tac
+ ‘?phi0. !phi. 
+  (Inj(phi) &
+  ghom(phi,Qg(g1,ker(f, g1, g2)),g2) &
+  phi o gqm(g1,ker(f, g1, g2)) = f) <=> phi = phi0’  
+ >-- cheat >> 
+ qby_tac
+ ‘!phi:Qc(g1,ker(f, g1, g2)) -> G2.
+    (Inj(phi) &
+    ghom(phi, Qg(g1, ker(f, g1, g2)), g2) &
+    phi o gqm(g1, ker(f, g1, g2)) = f) <=> 
+   (Inj(phi o Qctp(g1,K,ker(f, g1, g2))) &
+     ghom(phi o Qctp(g1,K,ker(f, g1, g2)), Qg(g1, K), g2) &
+    phi o Qctp(g1,K,ker(f, g1, g2)) o gqm(g1, K) = f)’ 
+ >-- cheat >> 
+ arw[] >>
+ qby_tac 
+ ‘!phi phi0:Qc(g1, ker(f, g1, g2))-> G2. phi = phi0 <=> 
+  phi o Qctp(g1,K, ker(f, g1, g2)) = phi0 o Qctp(g1,K, ker(f, g1, g2))’
+ >-- cheat >>
+ arw[] >>
+ qsuff_tac
+ ‘?psi0. !psi. 
+  (Inj(psi) &
+  ghom(psi,Qg(g1,K),g2) &
+  psi o gqm(g1,K) = f) <=> psi = psi0’ 
+ >-- (strip_tac >>
+     qexists_tac ‘psi0 o Qctp(g1,ker(f, g1, g2),K)’ >>
+     strip_tac >>
+     fs[GSYM o_assoc] >> rw[o_assoc] >> 
+     drule Qc_of_equal >>
+     arw[IdR]) >>
+ 
+
+
+
+ (*if have Makkai rule then everything is solved*)
+ pop_assum strip_assume_tac >>
+ qexists_tac ‘psi0 o Qctp(g1,ker(f, g1, g2),K)’ >>
+ strip_tac >> 
+ qby_tac 
+ ‘phi = psi0 o Qctp(g1, ker(f, g1, g2), K) <=> 
+  phi o Qctp(g1,K, ker(f, g1, g2)) = psi0’
+ >-- cheat >>
+ arw[] >> 
+ qby_tac
+ ‘!phi:Qc(g1,ker(f, g1, g2)) -> G2.
+    (Inj(phi) &
+    ghom(phi, Qg(g1, ker(f, g1, g2)), g2) &
+    phi o gqm(g1, ker(f, g1, g2)) = f) <=> 
+   (Inj(phi o Qctp(g1,K,ker(f, g1, g2))) &
+     ghom(phi o Qctp(g1,K,ker(f, g1, g2)), Qg(g1, K), g2) &
+    phi o Qctp(g1,K,ker(f, g1, g2)) o gqm(g1, K) = f)’ 
+ >-- cheat >>
+ arw[App_App_o] >>
+ first_x_assum
+ (qspecl_then [‘phi o Qctp(g1, K, ker(f, g1, g2))’]
+  assume_tac)>> 
+ fs[o_assoc]
+
+
+
+
+
+ qby_tac
+ ‘(!phi0 . (!phi.(Inj(phi) &
+    ghom(phi, Qg(g1, ker(f, g1, g2)), g2) &
+    phi o gqm(g1, ker(f, g1, g2)) = f) <=> phi = phi0)) ’
+ 
+
+ qsuff_tac
+ ‘?!psi. Inj(psi) &
+  ghom(psi,Qg(g1,K),g2) &
+  psi o gqm(g1,K) = f’
+ (*should be an iff*)
+ >-- strip_tac >> arw[] >>
+     
+
+ ‘!phi:Qc(g1,ker(f, g1, g2)) -> G2.
+  (Inj(phi) & 
+  ghom(phi, Qg(g1,K), g2) &
+  phi o gqm(g1,K) = f)’ <=> 
+  (Inj(phi o Qctp(g,K,ker(f, g1, g2))))’
+
+ qsuff_tac
+ ‘?!phi:Qc(g1,K) -> G2. 
+   Inj(phi) & 
+   ghom(phi, Qg(g1,K), g2) &
+   phi o gqm(g1,K) = f’
+ >-- strip_tac >>
+     qsuff_tac 
+     
+
+
+ qspecl_then [‘G1’,‘g1’,‘ker(f, g1, g2)’] assume_tac 
+ ER_cstR >>
+ drule Quot_UMP >>
+ qby_tac ‘resp1(f, cstR(g1, ker(f, g1, g2)))’ 
+ >-- cheat >>
+ first_x_assum drule >>
+ qby_tac ‘Quot(cstR(g1, ker(f, g1, g2)), 
+               iQc(g1,ker(f, g1, g2)))’ 
+ >-- cheat >>
+ first_x_assum drule >>
+ first_x_assum (qspecl_then [‘ecst(g1,ker(f, g1, g2))’]
+                            assume_tac) >>
+ qsuff_tac
+ ‘?phi.
+     Inj(phi) &
+     ghom(phi, Qg(g1, ker(f, g1, g2)), g2) &
+     phi o gqm(g1, ker(f, g1, g2)) = f’ 
+ >-- (strip_tac >> uex_tac >>
+     qexists_tac ‘phi’ >> arw[] >> rpt strip_tac >>
+     irule Surj_Epi >>
+     qexistsl_tac [‘G1’,‘gqm(g1, ker(f, g1, g2))’] >>
+     arw[gqm_Surj]) >> 
+ pop_assum (strip_assume_tac o uex2ex_rule) >>
+ qexists_tac ‘fb’ >>
+ qby_tac ‘fb o gqm(g1, ker(f, g1, g2)) = f’ 
+ >-- (rw[GSYM FUN_EXT,App_App_o] >> 
+     pop_assum (assume_tac o GSYM) >> arw[] >>
+     rw[gqm_def,GSYM abs_def]) >>
+ arw[] >>
+ qby_tac
+ ‘ghom(fb, Qg(g1, ker(f, g1, g2)), g2)’
+ >-- (rw[ghom_def] >> rpt strip_tac >> 
+     qsspecl_then [‘g1’,‘ker(f, g1, g2)’] assume_tac 
+     gqm_Surj >> fs[Surj_def] >>
+     first_assum 
+     (qspecl_then [‘a’]
+                  (x_choose_then "x" (assume_tac o GSYM))) >>
+     first_assum 
+     (qspecl_then [‘b’] 
+                  (x_choose_then "y" (assume_tac o GSYM))) >>
+     arw[] >> fs[gqm_Csof,gmul_Qg] >>
+     rw[GSYM gqm_Csof,GSYM App_App_o] >>arw[] >>
+     fs[ghom_def]) >>
+ arw[] >>
+ rw[Inj_def] >> rpt strip_tac >>
+ qsspecl_then [‘g1’,‘ker(f, g1, g2)’] assume_tac gqm_Surj >>
+ fs[Surj_def] >>
+ first_assum 
+ (qspecl_then [‘x1’]
+              (x_choose_then "a" (assume_tac o GSYM))) >>
+ first_assum 
+ (qspecl_then [‘x2’] 
+              (x_choose_then "b" (assume_tac o GSYM))) >>
+ arw[] >> fs[] >> 
+ pop_assum (K all_tac) >> pop_assum (K all_tac) >>
+ pop_assum (K all_tac) >>
+ rfs[GSYM App_App_o] >> 
+ rw[gqm_Csof] >>
+ qsuff_tac ‘IN(gmul(g1,a,ginv(g1,b)),ker(f,g1,g2))’ 
+ >-- cheat >>
+ rw[ker_def] >>
+ fs[ghom_def] >> last_x_assum (assume_tac o GSYM) >> arw[] >>
+ rw[gmul_ginv] >>
+ irule ghom_e >> arw[ghom_def])
+(form_goal “!G1 G2 f:G1->G2 g1 g2. 
+ ghom(f,g1,g2) & Surj(f) ==>
+ ?!phi:Qc(g1,ker(f,g1,g2)) -> G2. Inj(phi) & 
+ ghom(phi, Qg(g1,ker(f,g1,g2)), g2) &
+ phi o gqm(g1,ker(f,g1,g2)) = f”));
+
 
 val sgmul_def = proved_th $
 e0
@@ -293,10 +627,43 @@ cheat
  ?h k. IN(h,H) & IN(k,K) & hk = gmul(g,h,k)”)
 |> spec_all |> uex2ex_rule |> qSKOLEM "sgmul" [‘g’,‘H’,‘K’]
  
+val IM_def = qdefine_fsym("IM",[‘f:A->B’]) ‘IMAGE(f,Whole(A))’
+
+(*try this approach: for every subset, it can be regarded as a injection to the original set, this injection is unique up to iso in the cat of triangles, and therefore gives a function symbol Inc*)
+
+Thm_2_4 |> qspecl [‘A’] 
+|> fVar_sInst_th “P(a:mem(A))”
+   “IN(a,s:mem(Pow(A)))”
+|> qSKOLEM "Set" [‘s’] |> qSKOLEM "Inc" [‘s’]
+
+(*regard subgroup H as inc, then there is a group structure on Set(H) that makes it a group
+maybe abbr with equality is an issue suggests that should not use equality as abbrv, should be parsing/pp level stuff.
+ *)
+
+
+(*if H is given as a member of subgroup set, then can prove exists element of set H .*)
+
+val Set_sgrp_grp = proved_th $
+e0
+cheat
+(form_goal 
+ “!G g:mem(Grp(G)) H. issgrp(H,g) ==>
+  ?!h:mem(Grp(Set(H))).
+   Inc(H) o mof(h) = mof(g) o Prla(Inc(H),Inc(H)) &
+   Inc(H) o iof(h) = iof(g) &
+   App(Inc(H),eof(h)) = eof(g)”)
+ 
+(* H/H ∩ K ~ HK/K*)
 val second_iso_thm = prove_store("second_iso_thm",
 e0
 ()
-(form_goal “”));
+(form_goal 
+ “!G g H h:mem(Grp(H)) ih: H->G K k:mem(Grp(K)) ik:K->G. 
+  issgrp(IM(ih),g) & isnml(IM(ik),g) ==>
+  
+  
+  
+ ”));
 
 (*
 rastt "Qg(g1,H1:mem(Pow(G)))";
@@ -316,3 +683,4 @@ EQ_fsym "Qg" [refl(rastt "g1:mem(Grp(G))"),assume “H1 = H2:mem(Pow(G))”]
 “Qg(g1, H1) = Qg(g2,H2)”
 
 top_depth_conv (rewr_conv (assume “H1 = H2:mem(Pow(G))”)) (rastt "Qg(g1, H1:mem(Pow(G)))")
+*)
