SEARTree.sml
@@ -1,0 +1,354 @@
+val Lf0_def = qdefine_fsym("Lf0",[‘A’]) ‘injN(A,O)’
+
+(*
+val injN2U_def = proved_th $
+e0
+cheat
+(form_goal “∀A.∃!f:Pow(N * N * A) -> Pow(N * A).
+f = f”)
+|> spec_all |> uex2ex_rule |> qSKOLEM "injN2U" [‘A’]
+*)
+
+
+
+val Injopt_def = proved_th $
+e0
+(strip_tac >> irule
+ (P2fun_uex |> qspecl [‘A’,‘Pow(N * A)’] 
+ |> fVar_sInst_th “P(a0:mem(A),na:mem(Pow(N * A)))”
+    “(!n:mem(N) a:mem(A).IN(Pair(n,a),na) <=> a = a0)”) >>
+ strip_tac >> accept_tac
+ (IN_def_P |> qspecl [‘N * A’] 
+ |> fVar_sInst_th “P(na:mem(N * A))” “Snd(na:mem(N * A)) = x”
+ |> conv_rule (depth_fconv no_conv forall_cross_fconv)
+ |> rewr_rule[Pair_def']))
+(form_goal “!A. ?!injA:A + 1 -> Pow(N * A).
+ !a0. (!n a.IN(Pair(n,a),App(injA,a0)) <=> a = a0)”)
+|> spec_all |> uex2ex_rule |> qSKOLEM "InjA" [‘A’] |> gen_all 
+
+val injN2U_def = proved_th $
+e0
+cheat
+(form_goal “∀A f:N -> Pow(N * A).∃!f1: mem(Pow(N * A)).
+f1 = f1”)
+|> spec_all |> uex2ex_rule |> qSKOLEM "injN2U" [‘f’]
+
+(*
+val injN2U_def = 
+    qdefine_fsym("injN2U",[‘f:mem(Pow(N * N * A))’]) 
+                ‘App(InjN2U(A),f)’ 
+*)
+
+val Nd0_def = qdefine_fsym("Nd0",[‘n:mem(N)’,‘a:mem(A)’,
+ ‘f:N -> Pow(N * A)’]) ‘injUU(injN(A,Suc(n)),injUU(injA(a),injN2U(f)))’ 
+
+
+val f = 
+ “(nas = Lf0(A) ==> IN(nas,trees)) &
+  (!f. (!m.IN(App(f,m),trees)) ==>
+   !n a. IN(Nd0(n,a,f),trees))”
+
+val istree_cl = 
+ “(nas = Lf0(A) ==> IN(nas,istrees)) &
+  (!f n a. (!m.IN(App(f,m),istrees)) & nas = Nd0(n,a,f) ==>
+   IN(nas,istrees))”
+
+
+val (istree_incond,x1) = mk_incond istree_cl;
+val istreef_ex = mk_fex istree_incond x1;
+val istreef_def = mk_fdef "istreef" istreef_ex;
+val istreef_monotone = proved_th $
+e0
+cheat
+(form_goal
+ “!s1 s2. SS(s1,s2) ==>
+ SS(App(istreef(A),s1),App(istreef(A),s2))”);
+val istree's_def = mk_prim istreef_def;
+val istrees_def = mk_LFP (rastt "istree's(A)");
+val istrees_cond = mk_cond istrees_def istree's_def;
+val istrees_SS = mk_SS istrees_def istree's_def;
+val istree_rules0 = mk_rules istreef_monotone istrees_SS istrees_cond;
+val istree_cases0 = mk_cases istreef_monotone istree_rules0 istrees_cond;
+val istree_ind0 = mk_ind istrees_cond;
+val istree_ind1 = mk_ind1 istreef_def istree_ind0;
+val istree_ind2 = mk_ind2 istree_ind1;
+val istree_cases1 = mk_case1 istreef_def istree_cases0;
+val istree_rules1 = mk_rules1 istreef_def istree_rules0;
+val istree_rules2 = mk_rules2 istree_rules1;
+val istree_rules3 = mk_rules3 istree_rules2;
+
+
+
+val istree_ind = istree_ind2 |> store_as "istree_ind";
+val istree_cases = istree_cases1 |> store_as "istree_cases";
+val istree_rules = istree_rules3 |> store_as "istree_rules";
+
+
+
+val Tree_def = Thm_2_4  |> qspecl [‘Pow(N * A)’]
+                         |> fVar_sInst_th “P(f:mem(Pow(N * A)))”
+                         “istree(f:mem(Pow(N * A)))”
+                         |> qSKOLEM "Tree" [‘A’]
+                         |> qSKOLEM "iT" [‘A’]
+                         |> gen_all
+
+
+val iT_Inj = recsp_def |> spec_all 
+                      |> conjE1 |> gen_all
+                      |> store_as "iT_Inj"; 
+
+
+val istree_def = qdefine_psym("istree",[‘t:mem(Pow(N * A))’])
+‘IN(t,istrees(A))’ |> gen_all 
+
+
+val istree_induct = prove_store("istree_induct",
+e0
+(rw[istree_def] >> strip_tac >>
+ x_choose_then "s" (assume_tac o conjE1) 
+ (IN_def_P_expand |> qspecl [‘Pow(N * A)’]) >> arw[] >>
+ arw[istree_ind])
+(form_goal 
+ “!A.P(Lf0(A)) & 
+  (!f n a:mem(A). (!m.P(App(f,m))) ==>
+    P(Nd0(n,a,f))) ==>
+  !f0:mem(Pow(N * A)). istree(f0) ==> P(f0)”));
+ 
+
+val istree_Lf0 = prove_store("istree_Lf0",
+e0
+(rw[istree_def,istree_rules])
+(form_goal
+ “!A. istree(Lf0(A))”)); 
+
+
+val istree_Nd0 = istree_rules |> spec_all |> conjE2 
+                        |> rewr_rule[GSYM istree_def]
+                        |> spec_all |> undisch 
+                        |> gen_all |> disch_all
+                        |> gen_all |> store_as "istree_Nd0";
+
+
+val Rept_def = qdefine_fsym ("Rept",[‘t:mem(Tree(A))’])
+                            ‘App(iT(A),t)’
+                            |> gen_all |> store_as "Rept_def";
+
+val Rept_eq_eq = prove_store("Rept_eq_eq",
+e0
+(cheat)
+(form_goal “!A t1:mem(Tree(A)) t2.Rept(t1) = Rept(t2) <=> t1 = t2”));
+ 
+val Lf_def = proved_th $
+e0
+(strip_tac >> uex_tac >>
+ qspecl_then [‘A’] strip_assume_tac Tree_def >>
+ first_assum (qspecl_then [‘Lf0(A)’] assume_tac) >>
+ fs[istree_Lf0,GSYM istree_def] >>
+ qexists_tac ‘b’ >> arw[Rept_def] >>
+ fs[Inj_def])
+(form_goal “!A. ?!t.Rept(t) = Lf0(A)”)
+|> spec_all |> uex2ex_rule |> qSKOLEM "Lf" [‘A’] |> gen_all
+|> store_as "Lf_def";
+
+
+val istree_Rept = Tree_def |> spec_all |> conjE2
+                        |> rewr_rule[GSYM istree_def,
+                                     GSYM Rept_def] 
+                        |> gen_all 
+                        |> store_as "istree_Rept";
+
+val Nd_def = proved_th $
+e0
+(rpt strip_tac >>
+qsuff_tac ‘?nd0. Nd0(n,a,iT(A) o f) = Rept(nd0)’
+>-- (strip_tac >> uex_tac >> qexists_tac ‘nd0’ >>
+    arw[] >> rpt strip_tac >> fs[Rept_eq_eq]) >>
+rw[GSYM istree_Rept] >>
+irule istree_Nd0 >> rw[istree_Rept,Rept_def,App_App_o] >>
+rpt strip_tac >> qexists_tac ‘App(f,m)’ >> rw[])
+(form_goal
+“!n a f:N -> Tree(A). ?!nd0. 
+ Nd0(n,a,iT(A) o f) = Rept(nd0)”)
+|> spec_all |> uex2ex_rule |> qSKOLEM "Nd" [‘n’,‘a’,‘f’]
+
+(*
+val Rept_istree = prove_store("Rept_istree",
+e0
+()
+(form_goal “!t:mem(Tree(A)). istree(Rept)”));
+*)
+
+
+val Rept_Lf0_uex = prove_store("Rept_Lf0_uex",
+e0
+(rpt strip_tac >> dimp_tac >> strip_tac >> arw[Lf_def] >>
+ rw[GSYM Rept_eq_eq] >> arw[Lf_def])
+(form_goal
+ “!A t. Rept(t) = Lf0(A) <=> t = Lf(A)”));
+
+
+val Tree_induct = prove_store("Tree_induct",
+e0
+(strip_tac >> disch_tac >>
+ qsuff_tac ‘!nas:mem(Pow(N * A)). istree(nas) ==> istree(nas) &
+ (!t. Rept(t) = nas ==> P(t))’
+ >-- (strip_tac >>
+     qby_tac ‘!nas:mem(Pow(N * A)). istree(nas) ==>
+                      (!t. Rept(t) = nas ==> P(t))’ 
+     >-- (rpt strip_tac >> first_x_assum drule >>
+          rfs[] >> first_x_assum irule >> arw[]) >>
+     strip_tac >> first_x_assum irule >>
+     qexists_tac ‘Rept(t)’ >> rw[istree_Rept] >>
+     qexists_tac ‘t’ >> rw[]) >>
+ ind_with (istree_induct |> qspecl [‘A’]) >>
+ rw[istree_Lf0] >> strip_tac (* 2 *)
+ >-- (rpt strip_tac >>
+     qsuff_tac ‘t = Lf(A)’ >-- (strip_tac >> arw[]) >>
+     irule $ iffLR Rept_Lf0_uex >> arw[]) >>
+ rpt gen_tac >> disch_tac >>
+ pop_assum strip_assume_tac >>
+ qby_tac ‘istree(Nd0(n, a, f))’ 
+ >-- (irule istree_Nd0 >> arw[]) >> arw[] >>
+ rpt strip_tac >>
+ qby_tac ‘?f0. f = iT(A) o f0’ 
+ >-- cheat (*use assumption !(m : mem(N)).
+               istree(App(f, m#))  ...*)>>
+ pop_assum strip_assume_tac >> 
+ qsuff_tac ‘t = Nd(n,a,f0)’ 
+ >-- (strip_tac  >> last_x_assum strip_assume_tac >>
+      arw[] >> first_x_assum irule >> arw[] >>
+      rpt strip_tac >>
+      fs[App_App_o] >>
+      first_x_assum (qspecl_then [‘m’] strip_assume_tac) >>
+      first_x_assum irule >> rw[Rept_def]) >>
+ rw[GSYM Rept_eq_eq] >> arw[GSYM Nd_def])
+(form_goal
+ “!A. P(Lf(A)) & 
+      (!n a:mem(A) f.(!m.P(App(f,m))) ==> P(Nd(n,a,f))) ==>
+  !t:mem(Tree(A)).P(t) ”));
+
+(*tree-tuple*)
+val Fnap_def = qdefine_fsym("Fnap",[‘Fn:N * A * Exp(N,Tree(A)) * Exp(N,X) ->X’,‘n:mem(N)’,‘a:mem(A)’,‘f:N->Tree(A)’,‘y:N ->X’]) ‘App(Fn,Pair(n,Pair(a,Pair(Tpm(f),Tpm(y)))))’
+
+
+local
+val Tind_cl = 
+ “(p = Pair(Lf(A),l:mem(X)) ==> IN(p,Tind)) &
+  (!n a f:N->Tree(A) y. 
+   (!m.IN(Pair(App(f,m),App(y,m)),Tind)) &
+   p = Pair(Nd(n,a,f),Fnap(Fn,n,a,f,y)) ==>
+   IN(p,Tind))”
+in
+val (Tind_incond,x1) = mk_incond Tind_cl;
+val Tindf_ex = mk_fex Tind_incond x1;
+val Tindf_def = mk_fdef "Tindf" Tindf_ex;
+val Tindf_monotone = proved_th $
+e0
+cheat
+(form_goal
+ “!s1 s2. SS(s1,s2) ==>
+ SS(App(Tindf(Fn:N * A * Exp(N,Tree(A)) * Exp(N,X) ->X,l:mem(X)),s1),App(Tindf(Fn,l),s2))”);
+val Tind's_def = mk_prim Tindf_def;
+val Tinds_def = mk_LFP (rastt "Tind's(Fn:N * A * Exp(N,Tree(A)) * Exp(N,X) ->X,l:mem(X))");
+val Tinds_cond = mk_cond Tinds_def Tind's_def;
+val Tinds_SS = mk_SS Tinds_def Tind's_def;
+val Tind_rules0 = mk_rules Tindf_monotone Tinds_SS Tinds_cond;
+val Tind_cases0 = mk_cases Tindf_monotone Tind_rules0 Tinds_cond;
+val Tind_ind0 = mk_ind Tinds_cond;
+val Tind_ind1 = mk_ind1 Tindf_def Tind_ind0;
+val Tind_ind2 = mk_ind2 Tind_ind1; 
+val Tind_cases1 = mk_case1 Tindf_def Tind_cases0; 
+val Tind_rules1 = mk_rules1 Tindf_def Tind_rules0; 
+val Tind_rules2 = mk_rules2 Tind_rules1; 
+val Tind_rules3 = mk_rules3 Tind_rules2;
+end
+
+val Tind_ind = Tind_ind2 |> store_as "Tind_ind";
+val Tind_cases = Tind_cases1 |> store_as "Tind_cases";
+val Tind_rules = Tind_rules3 |> store_as "Tind_rules";
+
+val Nd_NONLF = prove_store("Nd_NONLF",
+e0
+cheat
+(form_goal “!A n a f . ~(Nd(n,a,f) = Lf(A))”));
+
+val Nd_eq_eq = prove_store("Nd_eq_eq",
+e0
+(cheat)
+(form_goal “!A n1 a1:mem(A) f1 n2 a2 f2.
+  Nd(n1,a1,f1) = Nd(n2,a2,f2) <=> n1 = n2 & a1 = a2 & f1 = f2 ”));
+
+val Tind_uex = prove_store("Tind_uex",
+e0
+(strip_tac >> strip_tac >> strip_tac >> strip_tac >>
+ ind_with (Tree_induct |> qspecl [‘A’]) >> strip_tac (* 2 *)
+ >-- (uex_tac >> qexists_tac ‘l’ >>
+      rw[Tind_rules] >> once_rw[Tind_cases] >>
+      rw[Pair_eq_eq,GSYM Nd_NONLF] >> rpt strip_tac) >>
+ rpt strip_tac >> uex_tac >>
+ qby_tac
+ ‘?j:N->X. !n. IN(Pair(App(f,n),App(j,n)),Tinds(Fn,l))’
+ >-- cheat >>
+ pop_assum strip_assume_tac >>
+ drule (Tind_rules |> conjE2 |> spec_all 
+                   |> undisch |> gen_all
+                   |> disch_all) >> 
+ qexists_tac ‘Fnap(Fn, n, a, f, j)’ >> arw[] >>
+ rpt strip_tac >> drule $ iffLR Tind_cases >>
+ fs[Pair_eq_eq,Nd_NONLF,Nd_eq_eq] >>
+ qby_tac ‘y = j’ >>
+ fs[] >> cheat)
+(form_goal “!X l:mem(X) A  Fn  t:mem(Tree(A)). ?!e. IN(Pair(t,e),Tinds(Fn,l))”));
+
+
+val Trec_def = P2fun' |> qspecl [‘Tree(A)’,‘X’] 
+                      |> fVar_sInst_th “P(t:mem(Tree(A)),
+                                          x:mem(X))”
+                          “IN(Pair(t:mem(Tree(A)),x),
+                              Tinds(Fn,l:mem(X)))”
+                      |> C mp (Tind_uex |> spec_all
+                                        |> qgen ‘t’)
+                      |> qSKOLEM "Trec" [‘Fn’,‘l’]
+                      |> qgenl [‘X’,‘l’,‘A’,‘Fn’]
+                      |> store_as "Trec_def";
+
+
+
+val Trec_Lf = prove_store("Trec_Lf",
+e0
+(rpt strip_tac >>
+ qsspecl_then [‘l’,‘Fn’,‘Lf(A)’] assume_tac Trec_def >>
+ drule $ iffLR Tind_cases >>
+ fs[Pair_eq_eq,GSYM Nd_NONLF])
+(form_goal “!X l:mem(X) A  Fn. 
+ App(Trec(Fn,l),Lf(A)) = l”));
+
+
+val App_Trec_Tinds = prove_store("App_Trec_Tinds",
+e0
+(rpt strip_tac >> dimp_tac >> strip_tac >--
+(pop_assum (assume_tac o GSYM) >> arw[Trec_def]) >>
+qsspecl_then [‘l’,‘Fn’,‘t’] assume_tac Trec_def >>
+qsspecl_then [‘l’,‘Fn’,‘t’] assume_tac Tind_uex >>
+pop_assum (strip_assume_tac o uex_expand) >>
+first_assum rev_drule >> arw[] >>
+first_assum irule >> arw[])
+(form_goal “!X l:mem(X) A  Fn.
+!t:mem(Tree(A)) x. App(Trec(Fn,l),t) = x <=> 
+IN(Pair(t,x),Tinds(Fn,l))”));
+
+
+val Trec_Nd = prove_store("Trec_Nd",
+e0
+(rpt strip_tac >>
+ qsspecl_then [‘l’,‘Fn’,‘Nd(n,a,f)’] assume_tac Trec_def >>
+ drule $ iffLR Tind_cases >> 
+ fs[Pair_eq_eq,Nd_NONLF,Nd_eq_eq] >>
+ qsuff_tac ‘y = Trec(Fn, l) o f'’ 
+ >-- (strip_tac >> arw[]) >>
+ flip_tac >> irule $ iffLR FUN_EXT >>
+ rw[App_App_o] >>  arw[App_Trec_Tinds])
+(form_goal “!X l:mem(X) A  Fn n a:mem(A) f. 
+ App(Trec(Fn,l),Nd(n,a,f)) = 
+ Fnap(Fn,n,a,f,Trec(Fn,l) o f)”));
+
